Source/Core/Helpers.cs
@@ -1,0 +1,305 @@
+using System;
+using System.Diagnostics.Contracts;
+
+namespace Microsoft.Boogie
+{
+  public class Helpers
+  {
+    public static string BeautifyBplString(string s)
+    {
+      Contract.Requires(s != null);
+      Contract.Ensures(Contract.Result<string>() != null);
+      // strip "^" if it is the first character, change "$result" to "result"
+      if (s.StartsWith("^") || s == "$result")
+      {
+        s = s.Substring(1);
+      }
+      else if (s.StartsWith("call"))
+      {
+        s = s.Substring(s.IndexOf('@') + 1);
+        if (s.StartsWith("formal@"))
+        {
+          s = "(value of formal parameter: " + s.Substring(7) + ")";
+        }
+      }
+
+      // strip "$in" from the end of identifier names
+      if (s.EndsWith("$in"))
+      {
+        return "(initial value of: " + s.Substring(0, s.Length - 3) + ")";
+      }
+      else
+      {
+        return s;
+      }
+    }
+
+    public static string PrettyPrintBplExpr(Expr e)
+    {
+      Contract.Requires(e != null);
+      Contract.Ensures(Contract.Result<string>() != null);
+      // anything that is unknown will just be printed via ToString
+      // OldExpr and QuantifierExpr, BvExtractExpr, BvConcatExpr are ignored for now
+      // LiteralExpr is printed as itself by ToString
+      if (e is IdentifierExpr)
+      {
+        string s = e.ToString();
+        return Helpers.BeautifyBplString(s);
+      }
+      else if (e is NAryExpr)
+      {
+        NAryExpr ne = (NAryExpr) e;
+        IAppliable fun = ne.Fun;
+        var eSeq = ne.Args;
+        if (fun != null)
+        {
+          if ((fun.FunctionName == "$Length" || fun.FunctionName == "$StringLength") && eSeq.Count == 1)
+          {
+            Expr e0 = eSeq[0];
+            if (e0 != null)
+            {
+              string s0 = PrettyPrintBplExpr(e0);
+              return s0 + ".Length";
+            }
+
+            //unexpected, just fall outside to the default
+          }
+          else if (fun.FunctionName == "$typeof" && eSeq.Count == 1)
+          {
+            Expr e0 = eSeq[0];
+            if (e0 != null)
+            {
+              string s0 = PrettyPrintBplExpr(e0);
+              return "(the dynamic type of: " + s0 + ")";
+            }
+
+            //unexpected, just fall outside to the default
+          }
+          else if (fun.FunctionName == "IntArrayGet" && eSeq.Count == 2)
+          {
+            Expr e0 = eSeq[0];
+            Expr e1 = eSeq[1];
+            if (e0 != null && e1 != null)
+            {
+              string s0 = PrettyPrintBplExpr(e0);
+              string s1 = PrettyPrintBplExpr(e1);
+              return s0 + "[" + s1 + "]";
+            }
+
+            //unexpected, just fall outside to the default
+          }
+          else if (fun.FunctionName == "$Is" && eSeq.Count == 2)
+          {
+            Expr e0 = eSeq[0];
+            Expr e1 = eSeq[1];
+            if (e0 != null && e1 != null)
+            {
+              string s0 = PrettyPrintBplExpr(e0);
+              string s1 = PrettyPrintBplExpr(e1);
+              return "(" + s0 + " == null || (" + s0 + " is " + s1 + "))";
+            }
+
+            //unexpected, just fall outside to the default
+          }
+          else if (fun.FunctionName == "$IsNotNull" && eSeq.Count == 2)
+          {
+            Expr e0 = eSeq[0];
+            Expr e1 = eSeq[1];
+            if (e0 != null && e1 != null)
+            {
+              string s0 = PrettyPrintBplExpr(e0);
+              string s1 = PrettyPrintBplExpr(e1);
+              return "(" + s0 + " is " + s1 + ")";
+            }
+
+            //unexpected, just fall outside to the default
+          }
+          else if (fun is MapSelect && eSeq.Count <= 3)
+          {
+            // only maps with up to two arguments are supported right now (here)
+            if (cce.NonNull(eSeq[0]).ToString() == "$Heap")
+            {
+              //print Index0.Index1, unless Index1 is "$elements", then just print Index0
+              string s0 = PrettyPrintBplExpr(cce.NonNull(eSeq[1]));
+              if (eSeq.Count > 2)
+              {
+                string s1 = PrettyPrintBplExpr(cce.NonNull(eSeq[2]));
+                if (s1 == "$elements")
+                {
+                  return s0;
+                }
+                else
+                {
+                  if (eSeq[2] is IdentifierExpr)
+                  {
+                    // strip the class name out of a fieldname
+                    s1 = s1.Substring(s1.LastIndexOf('.') + 1);
+                  }
+
+                  return s0 + "." + s1;
+                }
+              }
+            }
+
+            //unexpected, just fall outside to the default
+          }
+          else if (fun is Microsoft.Boogie.BinaryOperator && eSeq.Count == 2)
+          {
+            Microsoft.Boogie.BinaryOperator f = (Microsoft.Boogie.BinaryOperator) fun;
+            Expr e0 = eSeq[0];
+            Expr e1 = eSeq[1];
+            if (e0 != null && e1 != null)
+            {
+              string s0 = PrettyPrintBplExpr(e0);
+              string s1 = PrettyPrintBplExpr(e1);
+              string op = "";
+              switch (f.Op)
+              {
+                case Microsoft.Boogie.BinaryOperator.Opcode.Add:
+                  op = " + ";
+                  break;
+                case Microsoft.Boogie.BinaryOperator.Opcode.And:
+                  op = " && ";
+                  break;
+                case Microsoft.Boogie.BinaryOperator.Opcode.Div:
+                  op = " div ";
+                  break;
+                case Microsoft.Boogie.BinaryOperator.Opcode.Eq:
+                  op = " == ";
+                  break;
+                case Microsoft.Boogie.BinaryOperator.Opcode.Ge:
+                  op = " >= ";
+                  break;
+                case Microsoft.Boogie.BinaryOperator.Opcode.Gt:
+                  op = " > ";
+                  break;
+                case Microsoft.Boogie.BinaryOperator.Opcode.Iff:
+                  op = " <==> ";
+                  break;
+                case Microsoft.Boogie.BinaryOperator.Opcode.Imp:
+                  op = " ==> ";
+                  break;
+                case Microsoft.Boogie.BinaryOperator.Opcode.Le:
+                  op = " <= ";
+                  break;
+                case Microsoft.Boogie.BinaryOperator.Opcode.Lt:
+                  op = " < ";
+                  break;
+                case Microsoft.Boogie.BinaryOperator.Opcode.Mod:
+                  op = " mod ";
+                  break;
+                case Microsoft.Boogie.BinaryOperator.Opcode.Mul:
+                  op = " * ";
+                  break;
+                case Microsoft.Boogie.BinaryOperator.Opcode.Neq:
+                  op = " != ";
+                  break;
+                case Microsoft.Boogie.BinaryOperator.Opcode.Or:
+                  op = " || ";
+                  break;
+                case Microsoft.Boogie.BinaryOperator.Opcode.Pow:
+                  op = " ** ";
+                  break;
+                case Microsoft.Boogie.BinaryOperator.Opcode.RealDiv:
+                  op = " / ";
+                  break;
+                case Microsoft.Boogie.BinaryOperator.Opcode.Sub:
+                  op = " - ";
+                  break;
+                case Microsoft.Boogie.BinaryOperator.Opcode.Subtype:
+                  op = " <: ";
+                  break;
+                default:
+                  op = " ";
+                  break;
+              }
+
+              return "(" + s0 + op + s1 + ")";
+            }
+
+            //unexpected, just fall outside to the default
+          }
+          else
+          {
+            string s = fun.FunctionName + "(";
+            for (int i = 0; i < eSeq.Count; i++)
+            {
+              Expr ex = eSeq[i];
+              Contract.Assume(ex != null);
+              if (i > 0)
+              {
+                s += ", ";
+              }
+
+              string t = PrettyPrintBplExpr(ex);
+              if (t.StartsWith("(") && t.EndsWith(")"))
+              {
+                t = t.Substring(1, t.Length - 2);
+              }
+
+              s += t;
+            }
+
+            s += ")";
+            return s;
+            //unexpected, just fall outside to the default
+          }
+        }
+      }
+
+      return e.ToString();
+    }
+
+    private static readonly DateTime StartUp = DateTime.UtcNow;
+
+    public static void ExtraTraceInformation(string point)
+    {
+      Contract.Requires(point != null);
+      if (CommandLineOptions.Clo.TraceTimes)
+      {
+        DateTime now = DateTime.UtcNow;
+        TimeSpan timeSinceStartUp = now - StartUp;
+        Console.WriteLine(">>> {0}   [{1} s]", point, timeSinceStartUp.TotalSeconds);
+      }
+    }
+
+    // Substitute @PROC@ in a filename with the given descName
+    public static string SubstituteAtPROC(string descName, string fileName)
+    {
+      Contract.Requires(fileName != null);
+      Contract.Requires(descName != null);
+      Contract.Ensures(Contract.Result<string>() != null);
+      System.Text.StringBuilder /*!*/
+        sb =
+          new System.Text.StringBuilder(descName.Length);
+      // quote the name, characters like ^ cause trouble in CMD
+      // while $ could cause trouble in SH
+      foreach (char c in descName)
+      {
+        if (Char.IsLetterOrDigit(c) || c == '.')
+        {
+          sb.Append(c);
+        }
+        else
+        {
+          sb.Append('_');
+        }
+      }
+
+      string pn = sb.ToString();
+      // We attempt to avoid filenames that are too long, but we only
+      // do it by truncating the @PROC@ replacement, which leaves unchanged
+      // any filename extension specified by the user.  We base our
+      // calculations on that there is at most one occurrence of @PROC@.
+      if (180 <= fileName.Length - 6 + pn.Length)
+      {
+        pn = pn.Substring(0, Math.Max(180 - (fileName.Length - 6), 0)) + "-n" +
+             System.Threading.Interlocked.Increment(ref sequenceId);
+      }
+
+      return fileName.Replace("@PROC@", pn);
+    }
+
+    private static int sequenceId = -1;
+  }
+}
