Source/Core/TokenTextWriter.cs
@@ -1,0 +1,482 @@
+using System;
+using System.Collections.Generic;
+using System.Diagnostics.Contracts;
+using System.IO;
+using System.Linq;
+
+namespace Microsoft.Boogie
+{
+  public class TokenTextWriter : IDisposable
+  {
+    string /*!*/
+      filename;
+
+    TextWriter /*!*/
+      writer;
+
+    [ContractInvariantMethod]
+    void ObjectInvariant()
+    {
+      Contract.Invariant(filename != null);
+      Contract.Invariant(writer != null);
+    }
+
+    bool setTokens = true;
+    int line = 1;
+    int col;
+    public bool UseForComputingChecksums;
+
+    private const int indent_size = 2;
+    private int most_recent_indent_level = 0;
+
+    protected string Indent(int level)
+    {
+      Contract.Ensures(Contract.Result<string>() != null);
+      most_recent_indent_level = level;
+      return new string(' ', (indent_size * level));
+    }
+
+
+    // Keywords, this array *must* be sorted
+    public static readonly string[] /*!*/
+      BplKeywords =
+      {
+        "assert",
+        "assume",
+        "axiom",
+        "bool",
+        "break",
+        "call",
+        "cast",
+        "const",
+        "else",
+        "ensures",
+        "exists",
+        "false",
+        "forall",
+        "free",
+        "function",
+        "goto",
+        "havoc",
+        "if",
+        "implementation",
+        "int",
+        "invariant",
+        "modifies",
+        "old",
+        "procedure",
+        "public",
+        "requires",
+        "return",
+        "returns",
+        "rmode",
+        "true",
+        "type",
+        "unique",
+        "var",
+        "where",
+        "while",
+      };
+
+    // "Pretty" printing: not very efficient, and not necessarily very pretty, but helps a bit 
+    private readonly bool pretty;
+
+    // The stack of writers in a current separator-block.
+    // The string is an optional identifier that allows you
+    // to not start a new indentation for e.g. "&&" in "a && b && c".
+    // When the pretty printing is finished, this should be empty.
+    Stack<KeyValuePair<string, List<TextWriter>>> wstk;
+
+    // The original writer: where everything should finally end up.
+    TextWriter actual_writer;
+
+    public bool push(string type = null)
+    {
+      if (pretty)
+      {
+        if (wstk == null)
+        {
+          wstk = new Stack<KeyValuePair<string, List<TextWriter>>>();
+          actual_writer = writer;
+        }
+
+        if (wstk.Count > 0 && wstk.Peek().Key == type && type != null)
+        {
+          sep();
+          return false; // don't actually pop this thing (send this bool to pop)
+        }
+        else
+        {
+          wstk.Push(new KeyValuePair<string, List<TextWriter>>(type, new List<TextWriter> { }));
+          sep();
+          return true; // this needs to be popped
+        }
+      }
+      else
+      {
+        return false;
+      }
+    }
+
+    public void pop(bool do_it = true)
+    {
+      if (pretty)
+      {
+        if (do_it)
+        {
+          List<TextWriter> ws = wstk.Pop().Value;
+          // try to figure out if you should insert line breaks between
+          // them or print them on one single line
+          // this breaks down when there are newlines inserted
+          List<String> ss = new List<String>();
+          int len = 0;
+          foreach (TextWriter w in ws)
+          {
+            foreach (String s in w.ToString().Split(new String[] {"\r\n", "\n"}, StringSplitOptions.None))
+            {
+              if (s.Length > 0)
+              {
+                ss.Add(s);
+                len += s.Length;
+                // len = Math.Max(len, s.Length);
+              }
+            }
+          }
+
+          // figure out which is the next writer to use
+          List<TextWriter> tw = wstk.Count > 0 ? wstk.Peek().Value : null;
+          string indent_string;
+          if (tw == null)
+          {
+            writer = actual_writer;
+            indent_string = new string(' ', indent_size * most_recent_indent_level + indent_size);
+          }
+          else
+          {
+            writer = tw.Last();
+            indent_string = new string(' ', indent_size);
+          }
+
+          // write the strings (we would like to know WHERE we are in the document here)
+          if (len > 80 /* - wstk.Count * 2 */)
+          {
+            for (int i = 0; i < ss.Count; i++)
+            {
+              if (i != ss.Count - 1)
+              {
+                writer.WriteLine(ss[i]);
+                writer.Write(indent_string);
+              }
+              else
+              {
+                writer.Write(ss[i]);
+              }
+            }
+          }
+          else
+          {
+            foreach (String s in ss)
+            {
+              writer.Write(s);
+            }
+          }
+        }
+      }
+    }
+
+    public void sep()
+    {
+      if (pretty)
+      {
+        List<TextWriter> ws = wstk.Peek().Value;
+
+        writer = new StringWriter();
+        wstk.Peek().Value.Add(writer);
+      }
+    }
+
+    private IToken /*!*/ CurrentToken
+    {
+      get
+      {
+        Contract.Ensures(Contract.Result<IToken>() != null);
+
+        Token token = new Token();
+        token.filename = filename;
+        token.line = line;
+        token.col = col;
+        return token;
+      }
+    }
+
+    public void SetToken(Absy absy)
+    {
+      Contract.Requires(absy != null);
+      this.SetToken(t => absy.tok = t);
+    }
+
+    public void SetToken(IfThenElse expr)
+    {
+      Contract.Requires(expr != null);
+      this.SetToken(t => expr.tok = t);
+    }
+
+    public void SetToken(Action<IToken> setter)
+    {
+      Contract.Requires(setter != null);
+      if (this.setTokens)
+      {
+        setter(this.CurrentToken);
+      }
+    }
+
+    public void SetToken(ref IToken tok)
+    {
+      Contract.Requires(tok != null);
+      if (this.setTokens)
+      {
+        tok = this.CurrentToken;
+      }
+    }
+
+    public static string SanitizeIdentifier(string name)
+    {
+      Contract.Requires(name != null);
+      Contract.Ensures(Contract.Result<string>() != null);
+      int index = Array.BinarySearch(TokenTextWriter.BplKeywords, name);
+      if (index >= 0)
+      {
+        return "\\" + name;
+      }
+      else if (name.Length > 2 && name[0] == 'b' && name[1] == 'v')
+      {
+        return int.TryParse(name.Substring(2), out var dummy) ? "\\" + name : name;
+      }
+      else if (name.Contains('@'))
+      {
+        return SanitizeIdentifier(name.Replace("@", "#AT#"));
+      }
+      else
+      {
+        return name;
+      }
+    }
+
+    public TokenTextWriter(string filename)
+      : this(filename, false)
+    {
+    }
+
+    public TokenTextWriter(string filename, bool pretty)
+      : base()
+    {
+      Contract.Requires(filename != null);
+      this.pretty = pretty;
+      this.filename = filename;
+      this.writer = new StreamWriter(filename);
+    }
+
+    public TokenTextWriter(string filename, bool setTokens, bool pretty)
+      : base()
+    {
+      Contract.Requires(filename != null);
+      this.pretty = pretty;
+      this.filename = filename;
+      this.writer = new StreamWriter(filename);
+      this.setTokens = setTokens;
+    }
+
+    public TokenTextWriter(string filename, TextWriter writer, bool setTokens, bool pretty)
+      : base()
+    {
+      Contract.Requires(writer != null);
+      Contract.Requires(filename != null);
+      this.pretty = pretty;
+      this.filename = filename;
+      this.writer = writer;
+      this.setTokens = setTokens;
+    }
+
+    public TokenTextWriter(string filename, TextWriter writer, bool pretty)
+      : base()
+    {
+      Contract.Requires(writer != null);
+      Contract.Requires(filename != null);
+      this.pretty = pretty;
+      this.filename = filename;
+      this.writer = writer;
+    }
+
+    public TokenTextWriter(TextWriter writer)
+      : this(writer, false)
+    {
+    }
+
+    public TokenTextWriter(TextWriter writer, bool pretty)
+      : base()
+    {
+      Contract.Requires(writer != null);
+      this.pretty = pretty;
+      this.filename = "<no file>";
+      this.writer = writer;
+    }
+
+    public void Write(string text)
+    {
+      Contract.Requires(text != null);
+      this.writer.Write(text);
+      this.col += text.Length;
+    }
+
+    public void WriteIndent(int level)
+    {
+      if (!UseForComputingChecksums)
+      {
+        this.Write(Indent(level));
+      }
+    }
+
+    public void Write(string text, params object[] args)
+    {
+      Contract.Requires(text != null);
+      this.Write(string.Format(text, args));
+    }
+
+    public void Write(int level, string text)
+    {
+      Contract.Requires(text != null);
+      this.WriteIndent(level);
+      this.Write(text);
+    }
+
+    public void Write(int level, string text, params object[] args)
+    {
+      Contract.Requires(text != null);
+      this.WriteIndent(level);
+      this.Write(text, args);
+    }
+
+    public void Write(Absy node, string text)
+    {
+      Contract.Requires(text != null);
+      Contract.Requires(node != null);
+      this.SetToken(node);
+      this.Write(text);
+    }
+
+    public void Write(Absy node, string text, params string[] args)
+    {
+      Contract.Requires(text != null);
+      Contract.Requires(node != null);
+      this.SetToken(node);
+      this.Write(text, args);
+    }
+
+    public void Write(Absy node, int level, string text)
+    {
+      Contract.Requires(text != null);
+      Contract.Requires(node != null);
+      this.WriteIndent(level);
+      this.SetToken(node);
+      this.Write(text);
+    }
+
+    public void Write(Absy node, int level, string text, params object[] args)
+    {
+      Contract.Requires(text != null);
+      Contract.Requires(node != null);
+      this.WriteIndent(level);
+      this.SetToken(node);
+      this.Write(text, args);
+    }
+
+    public void WriteLine()
+    {
+      this.writer.WriteLine();
+      this.line++;
+      this.col = 0;
+    }
+
+    public void WriteLine(string text)
+    {
+      Contract.Requires(text != null);
+      this.writer.WriteLine(text);
+      this.line++;
+      this.col = 0;
+    }
+
+    public void WriteText(string text)
+    {
+      Contract.Requires(text != null);
+      int processed = 0;
+      while (true)
+      {
+        int n = text.IndexOf('\n', processed);
+        if (n == -1)
+        {
+          this.writer.Write(text);
+          this.col += text.Length - processed;
+          return;
+        }
+
+        processed = n + 1;
+        this.line++;
+        this.col = 0;
+      }
+    }
+
+    public void WriteLine(string text, params object[] args)
+    {
+      Contract.Requires(text != null);
+      this.WriteLine(string.Format(text, args));
+    }
+
+    public void WriteLine(int level, string text)
+    {
+      Contract.Requires(text != null);
+      this.WriteIndent(level);
+      this.WriteLine(text);
+    }
+
+    public void WriteLine(int level, string text, params object[] args)
+    {
+      Contract.Requires(text != null);
+      this.WriteIndent(level);
+      this.WriteLine(text, args);
+    }
+
+    public void WriteLine(Absy node, string text)
+    {
+      Contract.Requires(text != null);
+      Contract.Requires(node != null);
+      this.SetToken(node);
+      this.WriteLine(text);
+    }
+
+    public void WriteLine(Absy node, int level, string text)
+    {
+      Contract.Requires(text != null);
+      Contract.Requires(node != null);
+      this.SetToken(node);
+      this.WriteLine(level, text);
+    }
+
+    public void WriteLine(Absy node, int level, string text, params object[] args)
+    {
+      Contract.Requires(text != null);
+      Contract.Requires(node != null);
+      this.SetToken(node);
+      this.WriteLine(level, text, args);
+    }
+
+    public void Close()
+    {
+      this.writer.Close();
+    }
+
+    public void Dispose()
+    {
+      this.Close();
+    }
+  }
+}
