Source/Core/Util.cs
@@ -1,810 +1,101 @@
 using System;
-using System.IO;
-using System.Diagnostics.Contracts;
 using System.Collections.Generic;
-using System.Linq;
 
 namespace Microsoft.Boogie
 {
-  public class TokenTextWriter : IDisposable
+  public static class Util
   {
-    string /*!*/
-      filename;
 
-    TextWriter /*!*/
-      writer;
-
-    [ContractInvariantMethod]
-    void ObjectInvariant()
+    public static string EscapeFilename(string fn)
     {
-      Contract.Invariant(filename != null);
-      Contract.Invariant(writer != null);
+      return fn.Replace(':', '-').Replace('/', '-').Replace('\\', '-');
+    }
+    
+    public static int GetHashCode<T1, T2>(T1 arg1, T2 arg2)
+    {
+      unchecked
+      {
+        return 31 * arg1.GetHashCode() + arg2.GetHashCode();
+      }
+    }
+    
+    public static int GetHashCode<T1, T2, T3>(T1 arg1, T2 arg2, T3 arg3)
+    {
+      unchecked
+      {
+        int hash = arg1.GetHashCode();
+        hash = 31 * hash + arg2.GetHashCode();
+        return 31 * hash + arg3.GetHashCode();
+      }
     }
 
-    bool setTokens = true;
-    int line = 1;
-    int col;
-    public bool UseForComputingChecksums;
-
-    private const int indent_size = 2;
-    private int most_recent_indent_level = 0;
-
-    protected string Indent(int level)
+    public static int GetHashCode<T1, T2, T3, T4>(T1 arg1, T2 arg2, T3 arg3, 
+      T4 arg4)
     {
-      Contract.Ensures(Contract.Result<string>() != null);
-      most_recent_indent_level = level;
-      return new string(' ', (indent_size * level));
+      unchecked
+      {
+        int hash = arg1.GetHashCode();
+        hash = 31 * hash + arg2.GetHashCode();
+        hash = 31 * hash + arg3.GetHashCode();
+        return 31 * hash + arg4.GetHashCode();
+      }
     }
-
-
-    // Keywords, this array *must* be sorted
-    public static readonly string[] /*!*/
-      BplKeywords =
-      {
-        "assert",
-        "assume",
-        "axiom",
-        "bool",
-        "break",
-        "call",
-        "cast",
-        "const",
-        "else",
-        "ensures",
-        "exists",
-        "false",
-        "forall",
-        "free",
-        "function",
-        "goto",
-        "havoc",
-        "if",
-        "implementation",
-        "int",
-        "invariant",
-        "modifies",
-        "old",
-        "procedure",
-        "public",
-        "requires",
-        "return",
-        "returns",
-        "rmode",
-        "true",
-        "type",
-        "unique",
-        "var",
-        "where",
-        "while",
-      };
-
-    // "Pretty" printing: not very efficient, and not necessarily very pretty, but helps a bit 
-    private readonly bool pretty;
-
-    // The stack of writers in a current separator-block.
-    // The string is an optional identifier that allows you
-    // to not start a new indentation for e.g. "&&" in "a && b && c".
-    // When the pretty printing is finished, this should be empty.
-    Stack<KeyValuePair<string, List<TextWriter>>> wstk;
-
-    // The original writer: where everything should finally end up.
-    TextWriter actual_writer;
-
-    public bool push(string type = null)
+    
+    public static int GetHashCode<T1, T2, T3, T4, T5>(T1 arg1, T2 arg2, T3 arg3, 
+      T4 arg4, T5 arg5)
     {
-      if (pretty)
+      unchecked
       {
-        if (wstk == null)
+        int hash = arg1.GetHashCode();
+        hash = 31 * hash + arg2.GetHashCode();
+        hash = 31 * hash + arg3.GetHashCode();
+        hash = 31 * hash + arg4.GetHashCode();
+        return 31 * hash + arg5.GetHashCode();
+      }
+    }
+    
+    /**
+     * A pure hash code implementation for strings, instead of the default implementation that returns different hash codes between program executions.
+     */
+    public static int GetDeterministicHashCode(this string str)
+    {
+      unchecked
+      {
+        int hash1 = (5381 << 16) + 5381;
+        int hash2 = hash1;
+
+        for (int i = 0; i < str.Length; i += 2)
         {
-          wstk = new Stack<KeyValuePair<string, List<TextWriter>>>();
-          actual_writer = writer;
+          hash1 = ((hash1 << 5) + hash1) ^ str[i];
+          if (i == str.Length - 1)
+          {
+            break;
+          }
+
+          hash2 = ((hash2 << 5) + hash2) ^ str[i + 1];
         }
 
-        if (wstk.Count > 0 && wstk.Peek().Key == type && type != null)
-        {
-          sep();
-          return false; // don't actually pop this thing (send this bool to pop)
-        }
-        else
-        {
-          wstk.Push(new KeyValuePair<string, List<TextWriter>>(type, new List<TextWriter> { }));
-          sep();
-          return true; // this needs to be popped
-        }
-      }
-      else
-      {
-        return false;
+        return hash1 + (hash2 * 1566083941);
       }
     }
-
-    public void pop(bool do_it = true)
+    
+    public static V GetOrCreate<K, V>(this IDictionary<K, V> dictionary, K key, Func<V> createValue)
     {
-      if (pretty)
-      {
-        if (do_it)
-        {
-          List<TextWriter> ws = wstk.Pop().Value;
-          // try to figure out if you should insert line breaks between
-          // them or print them on one single line
-          // this breaks down when there are newlines inserted
-          List<String> ss = new List<String>();
-          int len = 0;
-          foreach (TextWriter w in ws)
-          {
-            foreach (String s in w.ToString().Split(new String[] {"\r\n", "\n"}, StringSplitOptions.None))
-            {
-              if (s.Length > 0)
-              {
-                ss.Add(s);
-                len += s.Length;
-                // len = Math.Max(len, s.Length);
-              }
-            }
-          }
-
-          // figure out which is the next writer to use
-          List<TextWriter> tw = wstk.Count > 0 ? wstk.Peek().Value : null;
-          string indent_string;
-          if (tw == null)
-          {
-            writer = actual_writer;
-            indent_string = new string(' ', indent_size * most_recent_indent_level + indent_size);
-          }
-          else
-          {
-            writer = tw.Last();
-            indent_string = new string(' ', indent_size);
-          }
-
-          // write the strings (we would like to know WHERE we are in the document here)
-          if (len > 80 /* - wstk.Count * 2 */)
-          {
-            for (int i = 0; i < ss.Count; i++)
-            {
-              if (i != ss.Count - 1)
-              {
-                writer.WriteLine(ss[i]);
-                writer.Write(indent_string);
-              }
-              else
-              {
-                writer.Write(ss[i]);
-              }
-            }
-          }
-          else
-          {
-            foreach (String s in ss)
-            {
-              writer.Write(s);
-            }
-          }
-        }
-      }
-    }
-
-    public void sep()
-    {
-      if (pretty)
-      {
-        List<TextWriter> ws = wstk.Peek().Value;
-
-        writer = new StringWriter();
-        wstk.Peek().Value.Add(writer);
-      }
-    }
-
-    private IToken /*!*/ CurrentToken
-    {
-      get
-      {
-        Contract.Ensures(Contract.Result<IToken>() != null);
-
-        Token token = new Token();
-        token.filename = filename;
-        token.line = line;
-        token.col = col;
-        return token;
-      }
-    }
-
-    public void SetToken(Absy absy)
-    {
-      Contract.Requires(absy != null);
-      this.SetToken(t => absy.tok = t);
-    }
-
-    public void SetToken(IfThenElse expr)
-    {
-      Contract.Requires(expr != null);
-      this.SetToken(t => expr.tok = t);
-    }
-
-    public void SetToken(Action<IToken> setter)
-    {
-      Contract.Requires(setter != null);
-      if (this.setTokens)
-      {
-        setter(this.CurrentToken);
-      }
-    }
-
-    public void SetToken(ref IToken tok)
-    {
-      Contract.Requires(tok != null);
-      if (this.setTokens)
-      {
-        tok = this.CurrentToken;
-      }
-    }
-
-    public static string SanitizeIdentifier(string name)
-    {
-      Contract.Requires(name != null);
-      Contract.Ensures(Contract.Result<string>() != null);
-      int index = Array.BinarySearch(TokenTextWriter.BplKeywords, name);
-      if (index >= 0)
-      {
-        return "\\" + name;
-      }
-      else if (name.Length > 2 && name[0] == 'b' && name[1] == 'v')
-      {
-        return int.TryParse(name.Substring(2), out var dummy) ? "\\" + name : name;
-      }
-      else if (name.Contains('@'))
-      {
-        return SanitizeIdentifier(name.Replace("@", "#AT#"));
-      }
-      else
-      {
-        return name;
-      }
-    }
-
-    public TokenTextWriter(string filename)
-      : this(filename, false)
-    {
-    }
-
-    public TokenTextWriter(string filename, bool pretty)
-      : base()
-    {
-      Contract.Requires(filename != null);
-      this.pretty = pretty;
-      this.filename = filename;
-      this.writer = new StreamWriter(filename);
-    }
-
-    public TokenTextWriter(string filename, bool setTokens, bool pretty)
-      : base()
-    {
-      Contract.Requires(filename != null);
-      this.pretty = pretty;
-      this.filename = filename;
-      this.writer = new StreamWriter(filename);
-      this.setTokens = setTokens;
-    }
-
-    public TokenTextWriter(string filename, TextWriter writer, bool setTokens, bool pretty)
-      : base()
-    {
-      Contract.Requires(writer != null);
-      Contract.Requires(filename != null);
-      this.pretty = pretty;
-      this.filename = filename;
-      this.writer = writer;
-      this.setTokens = setTokens;
-    }
-
-    public TokenTextWriter(string filename, TextWriter writer, bool pretty)
-      : base()
-    {
-      Contract.Requires(writer != null);
-      Contract.Requires(filename != null);
-      this.pretty = pretty;
-      this.filename = filename;
-      this.writer = writer;
-    }
-
-    public TokenTextWriter(TextWriter writer)
-      : this(writer, false)
-    {
-    }
-
-    public TokenTextWriter(TextWriter writer, bool pretty)
-      : base()
-    {
-      Contract.Requires(writer != null);
-      this.pretty = pretty;
-      this.filename = "<no file>";
-      this.writer = writer;
-    }
-
-    public void Write(string text)
-    {
-      Contract.Requires(text != null);
-      this.writer.Write(text);
-      this.col += text.Length;
-    }
-
-    public void WriteIndent(int level)
-    {
-      if (!UseForComputingChecksums)
-      {
-        this.Write(Indent(level));
-      }
-    }
-
-    public void Write(string text, params object[] args)
-    {
-      Contract.Requires(text != null);
-      this.Write(string.Format(text, args));
-    }
-
-    public void Write(int level, string text)
-    {
-      Contract.Requires(text != null);
-      this.WriteIndent(level);
-      this.Write(text);
-    }
-
-    public void Write(int level, string text, params object[] args)
-    {
-      Contract.Requires(text != null);
-      this.WriteIndent(level);
-      this.Write(text, args);
-    }
-
-    public void Write(Absy node, string text)
-    {
-      Contract.Requires(text != null);
-      Contract.Requires(node != null);
-      this.SetToken(node);
-      this.Write(text);
-    }
-
-    public void Write(Absy node, string text, params string[] args)
-    {
-      Contract.Requires(text != null);
-      Contract.Requires(node != null);
-      this.SetToken(node);
-      this.Write(text, args);
-    }
-
-    public void Write(Absy node, int level, string text)
-    {
-      Contract.Requires(text != null);
-      Contract.Requires(node != null);
-      this.WriteIndent(level);
-      this.SetToken(node);
-      this.Write(text);
-    }
-
-    public void Write(Absy node, int level, string text, params object[] args)
-    {
-      Contract.Requires(text != null);
-      Contract.Requires(node != null);
-      this.WriteIndent(level);
-      this.SetToken(node);
-      this.Write(text, args);
-    }
-
-    public void WriteLine()
-    {
-      this.writer.WriteLine();
-      this.line++;
-      this.col = 0;
-    }
-
-    public void WriteLine(string text)
-    {
-      Contract.Requires(text != null);
-      this.writer.WriteLine(text);
-      this.line++;
-      this.col = 0;
-    }
-
-    public void WriteText(string text)
-    {
-      Contract.Requires(text != null);
-      int processed = 0;
-      while (true)
-      {
-        int n = text.IndexOf('\n', processed);
-        if (n == -1)
-        {
-          this.writer.Write(text);
-          this.col += text.Length - processed;
-          return;
-        }
-
-        processed = n + 1;
-        this.line++;
-        this.col = 0;
-      }
-    }
-
-    public void WriteLine(string text, params object[] args)
-    {
-      Contract.Requires(text != null);
-      this.WriteLine(string.Format(text, args));
-    }
-
-    public void WriteLine(int level, string text)
-    {
-      Contract.Requires(text != null);
-      this.WriteIndent(level);
-      this.WriteLine(text);
-    }
-
-    public void WriteLine(int level, string text, params object[] args)
-    {
-      Contract.Requires(text != null);
-      this.WriteIndent(level);
-      this.WriteLine(text, args);
-    }
-
-    public void WriteLine(Absy node, string text)
-    {
-      Contract.Requires(text != null);
-      Contract.Requires(node != null);
-      this.SetToken(node);
-      this.WriteLine(text);
-    }
-
-    public void WriteLine(Absy node, int level, string text)
-    {
-      Contract.Requires(text != null);
-      Contract.Requires(node != null);
-      this.SetToken(node);
-      this.WriteLine(level, text);
-    }
-
-    public void WriteLine(Absy node, int level, string text, params object[] args)
-    {
-      Contract.Requires(text != null);
-      Contract.Requires(node != null);
-      this.SetToken(node);
-      this.WriteLine(level, text, args);
-    }
-
-    public void Close()
-    {
-      this.writer.Close();
-    }
-
-    public void Dispose()
-    {
-      this.Close();
-    }
-  }
-
-  public class Helpers
-  {
-    public static string BeautifyBplString(string s)
-    {
-      Contract.Requires(s != null);
-      Contract.Ensures(Contract.Result<string>() != null);
-      // strip "^" if it is the first character, change "$result" to "result"
-      if (s.StartsWith("^") || s == "$result")
-      {
-        s = s.Substring(1);
-      }
-      else if (s.StartsWith("call"))
-      {
-        s = s.Substring(s.IndexOf('@') + 1);
-        if (s.StartsWith("formal@"))
-        {
-          s = "(value of formal parameter: " + s.Substring(7) + ")";
-        }
+      if (dictionary.TryGetValue(key, out var result)) {
+        return result;
       }
 
-      // strip "$in" from the end of identifier names
-      if (s.EndsWith("$in"))
-      {
-        return "(initial value of: " + s.Substring(0, s.Length - 3) + ")";
-      }
-      else
-      {
-        return s;
-      }
+      result = createValue();
+      dictionary[key] = result;
+      return result;
     }
-
-    public static string PrettyPrintBplExpr(Expr e)
-    {
-      Contract.Requires(e != null);
-      Contract.Ensures(Contract.Result<string>() != null);
-      // anything that is unknown will just be printed via ToString
-      // OldExpr and QuantifierExpr, BvExtractExpr, BvConcatExpr are ignored for now
-      // LiteralExpr is printed as itself by ToString
-      if (e is IdentifierExpr)
-      {
-        string s = e.ToString();
-        return Helpers.BeautifyBplString(s);
+    
+    public static uint BoundedMultiply(uint a, uint b) {
+      try {
+        return a * b;
+      } catch (OverflowException) {
+        return UInt32.MaxValue;
       }
-      else if (e is NAryExpr)
-      {
-        NAryExpr ne = (NAryExpr) e;
-        IAppliable fun = ne.Fun;
-        var eSeq = ne.Args;
-        if (fun != null)
-        {
-          if ((fun.FunctionName == "$Length" || fun.FunctionName == "$StringLength") && eSeq.Count == 1)
-          {
-            Expr e0 = eSeq[0];
-            if (e0 != null)
-            {
-              string s0 = PrettyPrintBplExpr(e0);
-              return s0 + ".Length";
-            }
-
-            //unexpected, just fall outside to the default
-          }
-          else if (fun.FunctionName == "$typeof" && eSeq.Count == 1)
-          {
-            Expr e0 = eSeq[0];
-            if (e0 != null)
-            {
-              string s0 = PrettyPrintBplExpr(e0);
-              return "(the dynamic type of: " + s0 + ")";
-            }
-
-            //unexpected, just fall outside to the default
-          }
-          else if (fun.FunctionName == "IntArrayGet" && eSeq.Count == 2)
-          {
-            Expr e0 = eSeq[0];
-            Expr e1 = eSeq[1];
-            if (e0 != null && e1 != null)
-            {
-              string s0 = PrettyPrintBplExpr(e0);
-              string s1 = PrettyPrintBplExpr(e1);
-              return s0 + "[" + s1 + "]";
-            }
-
-            //unexpected, just fall outside to the default
-          }
-          else if (fun.FunctionName == "$Is" && eSeq.Count == 2)
-          {
-            Expr e0 = eSeq[0];
-            Expr e1 = eSeq[1];
-            if (e0 != null && e1 != null)
-            {
-              string s0 = PrettyPrintBplExpr(e0);
-              string s1 = PrettyPrintBplExpr(e1);
-              return "(" + s0 + " == null || (" + s0 + " is " + s1 + "))";
-            }
-
-            //unexpected, just fall outside to the default
-          }
-          else if (fun.FunctionName == "$IsNotNull" && eSeq.Count == 2)
-          {
-            Expr e0 = eSeq[0];
-            Expr e1 = eSeq[1];
-            if (e0 != null && e1 != null)
-            {
-              string s0 = PrettyPrintBplExpr(e0);
-              string s1 = PrettyPrintBplExpr(e1);
-              return "(" + s0 + " is " + s1 + ")";
-            }
-
-            //unexpected, just fall outside to the default
-          }
-          else if (fun is MapSelect && eSeq.Count <= 3)
-          {
-            // only maps with up to two arguments are supported right now (here)
-            if (cce.NonNull(eSeq[0]).ToString() == "$Heap")
-            {
-              //print Index0.Index1, unless Index1 is "$elements", then just print Index0
-              string s0 = PrettyPrintBplExpr(cce.NonNull(eSeq[1]));
-              if (eSeq.Count > 2)
-              {
-                string s1 = PrettyPrintBplExpr(cce.NonNull(eSeq[2]));
-                if (s1 == "$elements")
-                {
-                  return s0;
-                }
-                else
-                {
-                  if (eSeq[2] is IdentifierExpr)
-                  {
-                    // strip the class name out of a fieldname
-                    s1 = s1.Substring(s1.LastIndexOf('.') + 1);
-                  }
-
-                  return s0 + "." + s1;
-                }
-              }
-            }
-
-            //unexpected, just fall outside to the default
-          }
-          else if (fun is Microsoft.Boogie.BinaryOperator && eSeq.Count == 2)
-          {
-            Microsoft.Boogie.BinaryOperator f = (Microsoft.Boogie.BinaryOperator) fun;
-            Expr e0 = eSeq[0];
-            Expr e1 = eSeq[1];
-            if (e0 != null && e1 != null)
-            {
-              string s0 = PrettyPrintBplExpr(e0);
-              string s1 = PrettyPrintBplExpr(e1);
-              string op = "";
-              switch (f.Op)
-              {
-                case Microsoft.Boogie.BinaryOperator.Opcode.Add:
-                  op = " + ";
-                  break;
-                case Microsoft.Boogie.BinaryOperator.Opcode.And:
-                  op = " && ";
-                  break;
-                case Microsoft.Boogie.BinaryOperator.Opcode.Div:
-                  op = " div ";
-                  break;
-                case Microsoft.Boogie.BinaryOperator.Opcode.Eq:
-                  op = " == ";
-                  break;
-                case Microsoft.Boogie.BinaryOperator.Opcode.Ge:
-                  op = " >= ";
-                  break;
-                case Microsoft.Boogie.BinaryOperator.Opcode.Gt:
-                  op = " > ";
-                  break;
-                case Microsoft.Boogie.BinaryOperator.Opcode.Iff:
-                  op = " <==> ";
-                  break;
-                case Microsoft.Boogie.BinaryOperator.Opcode.Imp:
-                  op = " ==> ";
-                  break;
-                case Microsoft.Boogie.BinaryOperator.Opcode.Le:
-                  op = " <= ";
-                  break;
-                case Microsoft.Boogie.BinaryOperator.Opcode.Lt:
-                  op = " < ";
-                  break;
-                case Microsoft.Boogie.BinaryOperator.Opcode.Mod:
-                  op = " mod ";
-                  break;
-                case Microsoft.Boogie.BinaryOperator.Opcode.Mul:
-                  op = " * ";
-                  break;
-                case Microsoft.Boogie.BinaryOperator.Opcode.Neq:
-                  op = " != ";
-                  break;
-                case Microsoft.Boogie.BinaryOperator.Opcode.Or:
-                  op = " || ";
-                  break;
-                case Microsoft.Boogie.BinaryOperator.Opcode.Pow:
-                  op = " ** ";
-                  break;
-                case Microsoft.Boogie.BinaryOperator.Opcode.RealDiv:
-                  op = " / ";
-                  break;
-                case Microsoft.Boogie.BinaryOperator.Opcode.Sub:
-                  op = " - ";
-                  break;
-                case Microsoft.Boogie.BinaryOperator.Opcode.Subtype:
-                  op = " <: ";
-                  break;
-                default:
-                  op = " ";
-                  break;
-              }
-
-              return "(" + s0 + op + s1 + ")";
-            }
-
-            //unexpected, just fall outside to the default
-          }
-          else
-          {
-            string s = fun.FunctionName + "(";
-            for (int i = 0; i < eSeq.Count; i++)
-            {
-              Expr ex = eSeq[i];
-              Contract.Assume(ex != null);
-              if (i > 0)
-              {
-                s += ", ";
-              }
-
-              string t = PrettyPrintBplExpr(ex);
-              if (t.StartsWith("(") && t.EndsWith(")"))
-              {
-                t = t.Substring(1, t.Length - 2);
-              }
-
-              s += t;
-            }
-
-            s += ")";
-            return s;
-            //unexpected, just fall outside to the default
-          }
-        }
-      }
-
-      return e.ToString();
-    }
-
-    private static readonly DateTime StartUp = DateTime.UtcNow;
-
-    public static void ExtraTraceInformation(string point)
-    {
-      Contract.Requires(point != null);
-      if (CommandLineOptions.Clo.TraceTimes)
-      {
-        DateTime now = DateTime.UtcNow;
-        TimeSpan timeSinceStartUp = now - StartUp;
-        Console.WriteLine(">>> {0}   [{1} s]", point, timeSinceStartUp.TotalSeconds);
-      }
-    }
-
-    // Substitute @PROC@ in a filename with the given descName
-    public static string SubstituteAtPROC(string descName, string fileName)
-    {
-      Contract.Requires(fileName != null);
-      Contract.Requires(descName != null);
-      Contract.Ensures(Contract.Result<string>() != null);
-      System.Text.StringBuilder /*!*/
-        sb =
-          new System.Text.StringBuilder(descName.Length);
-      // quote the name, characters like ^ cause trouble in CMD
-      // while $ could cause trouble in SH
-      foreach (char c in descName)
-      {
-        if (Char.IsLetterOrDigit(c) || c == '.')
-        {
-          sb.Append(c);
-        }
-        else
-        {
-          sb.Append('_');
-        }
-      }
-
-      string pn = sb.ToString();
-      // We attempt to avoid filenames that are too long, but we only
-      // do it by truncating the @PROC@ replacement, which leaves unchanged
-      // any filename extension specified by the user.  We base our
-      // calculations on that there is at most one occurrence of @PROC@.
-      if (180 <= fileName.Length - 6 + pn.Length)
-      {
-        pn = pn.Substring(0, Math.Max(180 - (fileName.Length - 6), 0)) + "-n" +
-             System.Threading.Interlocked.Increment(ref sequenceId);
-      }
-
-      return fileName.Replace("@PROC@", pn);
-    }
-
-    private static int sequenceId = -1;
-  }
-  
-  public class ListComparer<T> : IEqualityComparer<List<T>>
-  {
-    public bool Equals(List<T> l1, List<T> l2)
-    {
-      if (l1.Count != l2.Count)
-      {
-        return false;
-      }
-
-      for (int i = 0; i < l1.Count; i++)
-      {
-        if (!l1[i].Equals(l2[i]))
-        {
-          return false;
-        }
-      }
-
-      return true;
-    }
-
-    public int GetHashCode(List<T> l)
-    {
-      int hCode = 0;
-      l.Iter(x => { hCode = hCode ^ x.GetHashCode(); });
-      return hCode.GetHashCode();
     }
   }
 }
