Source/VCGeneration/Prune/AxiomVisitor.cs
@@ -1,4 +1,5 @@
 using System;
+using System.Collections.Generic;
 using System.Diagnostics.Contracts;
 using System.Linq;
 
@@ -17,8 +18,9 @@ namespace Microsoft.Boogie
     
     private void VisitTriggerCustom(Trigger t) {
       var visitor = new TriggerVisitor();
-      var triggerList = t.Tr.ToList();
-      triggerList.ForEach(e => visitor.VisitExpr(e));
+      foreach (var trigger in t.Tr) {
+        visitor.VisitExpr(trigger);
+      }
       var incomingSet = visitor.Declarations.ToArray();
       AddIncoming(incomingSet);
     }
@@ -54,8 +56,8 @@ namespace Microsoft.Boogie
           VisitTriggerCustom(start);
           start = start.Next;
         }
-        var discardBodyIncoming = (qe is ForallExpr fa && fa.pos == Expr.Position.Pos && qe.Triggers != null)
-                                  || qe is ExistsExpr ee && ee.pos == Expr.Position.Neg;
+        var discardBodyIncoming = (qe is ForallExpr { pos: Expr.Position.Pos } && qe.Triggers != null)
+                                  || (qe is ExistsExpr { pos: Expr.Position.Neg } && qe.Triggers != null);
         be.Body.pos = Expr.Position.Neither;
         if (discardBodyIncoming) {
           var incomingOld = incomingSets;
