Source/VCGeneration/Prune/BlocksVisitor.cs
@@ -5,17 +5,10 @@ namespace Microsoft.Boogie
   internal class BlocksVisitor : DependencyEvaluator
   {
     public List<Block> Blocks;
-    public HashSet<Variable> RelVars;
 
     public BlocksVisitor(List<Block> blocks) : base(null)
     {
       Blocks = blocks;
-      RelVars = new HashSet<Variable>();
-    }
-
-    public override Variable VisitVariable(Variable v) {
-      RelVars.Add(v);
-      return base.VisitVariable(v);
     }
 
     public override Expr VisitExpr(Expr node)
@@ -26,17 +19,6 @@ namespace Microsoft.Boogie
         AddOutgoing(f.Func);
       }
       return base.VisitExpr(node);
-    }
-
-    public override Cmd VisitAssumeCmd(AssumeCmd ac) {
-      if (Prune.GetWhereVariable(ac) != null) {
-        var cacheVars = new HashSet<Variable> (RelVars);
-        var ex = base.VisitAssumeCmd(ac);
-        this.RelVars = cacheVars;
-        return ex;
-      } else {
-        return base.VisitAssumeCmd(ac);
-      }
     }
 
     public override Boogie.Type VisitType(Boogie.Type node)
